Working on a refinement (r1) of abstract-multi-paxos.

Isabelle2/AbstractMultiPaxosR1.thy
@@ -1,19 +1,12 @@
-theory AbstractMultiPaxos7
-imports  "../../IO-Automata/IOA" BallotArrays3
+theory AbstractMultiPaxosR1
+imports  "../../IO-Automata/IOA" BallotArrays3 DistributedSafeAt
 begin
-
-section {* Definition of the Abstract MultiPaxos I/O-automaton *}
-
-subsection {* State and actions *}
-
-text {* The actions (labels on transitions) of the I/O-automaton *}
-
-text {* The states of the I/O-automaton *}
 
 record ('v,'a) amp_state =
   propCmd :: "'v set"
   ballot :: "'a \<Rightarrow> nat"
-  vote :: "nat \<Rightarrow> 'a \<Rightarrow> nat \<Rightarrow> 'v option"
+  vote :: "nat \<Rightarrow> 'a \<Rightarrow> nat \<rightharpoonup> 'v"
+  suggestion :: "nat \<Rightarrow> nat \<rightharpoonup> 'v"
 
 locale amp_ioa = IOA +
   fixes quorums::"'a set set"
@@ -27,13 +20,14 @@ datatype ('vv,'aa,'ll) amp_action =
 
 definition amp_asig where
   "amp_asig \<equiv>
-    \<lparr> inputs = {Propose c | c . True},
-      outputs = {Learn i v l | i v l . l \<in> learners},
+    \<lparr> inputs = { Propose c | c . True},
+      outputs = { Learn i v l | i v l . l \<in> learners},
       internals = {Internal}\<rparr>"
 
 definition amp_start where
   -- {* The initial state *}
-  "amp_start \<equiv> {\<lparr>propCmd = {}, ballot = (\<lambda> a . 0), vote = (\<lambda> i a b . None) \<rparr>}"
+  "amp_start \<equiv> {\<lparr>propCmd = {}, ballot = (\<lambda> a . 0), vote = (\<lambda> i a . Map.empty), 
+    suggestion = \<lambda> i . Map.empty \<rparr>}"
 
 subsection {* The transitions *}
 
@@ -46,18 +40,22 @@ definition join_ballot where
 
 abbreviation proved_safe_at where 
   -- {* v is proved safe in instance i at ballot b by quorum q *}
-  "proved_safe_at s i q b v \<equiv> ballot_array.proved_safe_at_2_a quorums (ballot s) (vote s i) q b v"
+  "proved_safe_at s i q b v \<equiv> distributed_safe_at.proved_safe_at (ballot s) (vote s i) quorums q b v"
 
 abbreviation conservative_at where
   "conservative_at s i \<equiv> ballot_array.conservative_array (vote s i)"
 
-definition do_vote where
-  "do_vote a i q v s s' \<equiv> let b = ballot s a in
-          v \<in> propCmd s
-        \<and> vote s i a b = None
+definition suggest where
+  "suggest i b v q s s' \<equiv>
+          v \<in> propCmd s 
+        \<and> suggestion s i b = None
         \<and> proved_safe_at s i q b v
-        \<and> q \<in> quorums
-        \<and> conservative_at s' i
+        \<and> s' = s\<lparr>suggestion := (suggestion s)(i := (suggestion s i)(b \<mapsto> v))\<rparr>"
+
+definition do_vote where
+  "do_vote a i v s s' \<equiv> let b = ballot s a in
+          vote s i a b = None
+        \<and> suggestion s i b = Some v
         \<and> s' = s\<lparr>vote := (vote s)(i := (vote s i)(a := (vote s i a)(b := Some v)))\<rparr>"
 
 abbreviation chosen where
@@ -69,16 +67,19 @@ definition learn where
 fun amp_trans_rel where
   "amp_trans_rel r (Propose c) r' = propose c r r'"
 | "amp_trans_rel r Internal r' = (
-    (\<exists> a b . join_ballot a b r r')
-    \<or> (\<exists> a q i v . do_vote a i q v r r'))"
+    (\<exists> a b . join_ballot a b r r') 
+    \<or> (\<exists> a i v . do_vote a i v r r')
+    \<or> (\<exists> i b v q . suggest i b v q r r'))"
 | "amp_trans_rel r (Learn i v l) r' = learn i v r r'"
+
 
 lemma trans_cases: assumes "amp_trans_rel r a r'"
   obtains 
   (propose) c where "propose c r r'"
 | (learn) i v where "learn i v r r'"
 | (join_ballot) a b where "join_ballot a b r r'"
-| (do_vote) a i q v where "do_vote a i q v r r'"
+| (do_vote) a i v where "do_vote a i v r r'"
+| (suggest) i b v q where "suggest i b v q r r'"
 using assms apply induct apply auto done
 
 definition amp_trans where
@@ -93,5 +94,6 @@ lemmas simps = amp_ioa_def amp_asig_def amp_start_def amp_trans_def propose_def 
   do_vote_def learn_def
 
 end
+
 
 end
