Isabelle2/AbstractMultiPaxosR1Correctness.thy
@@ -1,0 +1,157 @@
+section {* Proof of the agreement property of AbstractMultiPaxos. *}
+
+theory AbstractMultiPaxosR1Correctness
+imports AbstractMultiPaxosR1 "../../IO-Automata/Simulations" "../../IO-Automata/IOA_Automation"
+  BallotArrayProperties
+begin
+
+locale amp_proof = IOA + quorums quorums + amp_ioa quorums learners for
+     quorums :: "'a set set" and learners :: "'l set" +
+  fixes the_ioa :: "(('v,'a)amp_state, ('v,'a,'l)amp_action) ioa"
+  defines "the_ioa \<equiv> amp_ioa"
+begin
+
+subsection {* Automation setup and a few lemmas *}
+
+lemmas amp_ioa_defs =
+   is_trans_def actions_def amp_trans_def amp_start_def
+   externals_def amp_ioa_def amp_asig_def
+
+declare amp_ioa_defs[inv_proofs_defs]
+declare the_ioa_def[inv_proofs_defs]
+
+declare propose_def[simp] join_ballot_def[simp] do_vote_def[simp] suggest_def[simp]
+  learn_def[simp] Let_def[simp] split_if[split] split_if_asm[split]
+
+(*  Nitpick config:
+nitpick[no_assms, show_consts, verbose, card 'a = 3, card 'v = 2, card nat = 2, card "'v option" = 3, card "nat option" = 3,
+    card "('v \<times> nat) option" = 5, card "'v \<times> nat" = 4, card unit = 1, card "('v, 'a) amp_state" = 32]
+*)
+method rm_trans_rel_assm = 
+  (match premises in P[thin]:"amp_trans_rel ?x ?y ?z" \<Rightarrow> \<open>-\<close>)
+method unfold_to_trans_rel = 
+  (simp add:is_trans_def the_ioa_def amp_ioa_def amp_trans_def)
+
+definition inv1 where
+  -- {* acceptors only vote for the suggestion. *}
+  inv1_def[inv_proofs_defs]:"inv1 s \<equiv> \<forall> i a b . let v = vote s i a b in
+    v \<noteq> None \<longrightarrow> v = suggestion s i b"
+
+lemma inv1:
+  "invariant the_ioa inv1"
+apply (rule invariantI)
+apply (force simp add:inv_proofs_defs invs)
+apply (unfold_to_trans_rel)
+apply (rm_reachable)
+apply ((induct_tac rule:trans_cases, simp); rm_trans_rel_assm)
+apply (simp_all add:inv1_def)
+by (metis option.simps(3))
+declare inv1[invs]
+
+abbreviation safe_at where "safe_at s i \<equiv> ballot_array.safe_at quorums (ballot s) (vote s i)"
+
+declare 
+  ballot_array.conservative_array_def[inv_proofs_defs]
+  ballot_array.conservative_def[inv_proofs_defs]
+
+abbreviation conservative_array where
+"conservative_array s \<equiv>  \<forall> i . conservative_at s i"
+
+lemma conservative:
+  "invariant the_ioa conservative_array"
+apply (rule invariantI)
+apply (force simp add:inv_proofs_defs)
+apply instantiate_invs_2
+apply (unfold_to_trans_rel)
+apply (induct_tac rule:trans_cases, simp)
+apply (auto simp add:ballot_array.conservative_def)[3]
+defer
+apply (auto simp add:ballot_array.conservative_def)[1]
+subgoal premises prems using prems(1,3,5)  apply (simp add:inv_proofs_defs split add:option.splits) by metis
+done
+declare conservative[invs]
+
+lemma trans_imp_prefix_order:
+  assumes "s \<midarrow>a\<midarrow>the_ioa\<longrightarrow> t"
+  shows "is_prefix (ballot s) (ballot t) (vote s i) (vote t i)" using assms
+  apply (simp add:inv_proofs_defs)
+  apply (induct rule:trans_cases)
+  apply (auto simp add:is_prefix_def inv_proofs_defs split add:option.split_asm)
+done
+
+lemma safe_mono:
+  -- {* @{term safe_at} is monotonic. *}
+  assumes "s \<midarrow>a\<midarrow>the_ioa\<longrightarrow> t" and "safe_at s i v b"
+  shows "safe_at t i v b" using assms ballot_array_prefix.safe_at_mono
+by (metis ballot_array_prefix_axioms.intro ballot_array_prefix_def quorums_axioms trans_imp_prefix_order)
+
+definition inv2 where
+  -- {* a suggestion is safe. *}
+  inv2_def[inv_proofs_defs]:"inv2 s \<equiv> \<forall> i b . case suggestion s i b of Some v \<Rightarrow> safe_at s i v b | None \<Rightarrow> True"
+
+lemma inv2:
+  "invariant the_ioa inv2"
+apply (rule invariantI)
+apply (force simp add:inv_proofs_defs invs)
+apply (rm_reachable)
+subgoal premises prems for s t a
+proof -
+  from prems and safe_mono have 1:"\<And> i v b . safe_at s i v b \<Longrightarrow> safe_at t i v b"
+    by (simp add:inv2_def)
+  with prems show ?thesis
+  apply (unfold_to_trans_rel)
+  apply ((induct_tac rule:trans_cases, simp); rm_trans_rel_assm)
+  apply (auto simp add:inv_proofs_defs split add:option.splits)[3]
+  apply (fastforce simp add:inv_proofs_defs split add:option.splits)
+  (* TODO: here we need "conservative" *)
+  apply (cases s, auto simp add:inv2_def split add:option.splits) oops
+
+abbreviation safe where "safe s \<equiv> \<forall> i . ballot_array.safe  quorums (ballot s) (vote s i)"
+
+lemma safe_votes:
+  assumes "s \<midarrow>aa\<midarrow>the_ioa\<longrightarrow> t" and "vote s i a b  \<noteq> vote t i a b" and "vote t i a b = Some v"
+  and "conservative_array s" and "safe s"
+  shows "safe_at t i v b"
+using assms
+apply (auto simp add:inv_proofs_defs)
+apply (induct rule:trans_cases)
+apply (auto simp add:inv_proofs_defs split add:option.splits)
+subgoal premises prems
+  proof -
+    have "safe_at s i v (ballot s a)"  
+  qed
+done
+
+lemma safe_inv:
+  "invariant the_ioa safe" oops
+apply (try_solve_inv2 inv_proofs_defs:inv_proofs_defs ballot_array.safe_def invs:invs)
+subgoal premises prems for s t act
+proof (auto simp add:ballot_array.safe_def split add:option.splits)
+  fix i b a v
+  assume "vote t i a b = Some v"
+  show "safe_at t i v b"
+  proof (cases "vote s i a b = vote t i a b")
+    case True
+    hence "safe_at s i v b" using prems(1) by (metis \<open>vote t i a b = Some v\<close> ballot_array.safe_def option.simps(5))
+    thus ?thesis using prems(2) safe_mono by simp
+  next
+    case False thus ?thesis using safe_votes by (metis \<open>vote t i a b = Some v\<close> prems(1) prems(2) prems(3))
+  qed
+qed
+done
+declare safe_inv[invs]
+
+subsection {* Finally, the proof that agreement holds (trivial, follows immediately from safe). *}
+
+definition agreement where 
+  "agreement s \<equiv> \<forall> v w i . chosen s i v \<and> chosen s i w \<longrightarrow> v = w"
+
+lemma agreement:"invariant the_ioa agreement"
+apply(rule invariantI)
+    apply(auto simp add: inv_proofs_defs agreement_def ballot_array.chosen_def ballot_array.chosen_at_def)[1]
+  apply (metis (mono_tags, lifting) IOA.invariant_def IOA.reachable_n agreement_def amp_proof.safe_inv amp_proof_axioms ballot_array_props.intro ballot_array_props.safe_imp_agreement quorums_axioms the_ioa_def)
+done
+
+end
+
+end
